AwsCryptographicMaterialProviders/dafny/AwsCryptographicMaterialProviders/src/Keyrings/RawAESKeyring.dfy
@@ -504,7 +504,8 @@ module RawAESKeyring {
              MaterialWrapping.WrapInput(
                plaintextMaterial := plaintextMaterial,
                algorithmSuite := input.algorithmSuite,
-               encryptionContext := input.encryptionContext
+               encryptionContext := input.encryptionContext,
+               serializedEC := input.serializedEC
              ),
              Success(MaterialWrapping.WrapOutput(
                        wrappedMaterial := res.value.wrappedMaterial,
@@ -541,7 +542,8 @@ module RawAESKeyring {
         MaterialWrapping.WrapInput(
           plaintextMaterial := plaintextMaterial,
           algorithmSuite := input.algorithmSuite,
-          encryptionContext := input.encryptionContext
+          encryptionContext := input.encryptionContext,
+          serializedEC := input.serializedEC
         ), []);
 
       res := Success(MaterialWrapping.GenerateAndWrapOutput(
